Instances/Monad.v
@@ -1,7 +1,5 @@
 Require Export Base.
 Require Import Coq.Program.Basics.
-Require Import Classes.Applicative.
-Require Import Classes.Functor.
 Require Export Classes.Monad.
 Require Import FunctionalExtensionality.
 Require Import Language.Statements.
@@ -15,95 +13,6 @@ Inductive Maybe A : Type :=
     | None : Maybe A.
 Arguments Just {_}.
 Arguments None {_}.
-
-Section Maybe_Functor.
-  Definition fmap_maybe {A B} (f : A → B) ma : Maybe B :=
-    match ma with
-    | Just a => Just (f a)
-    | None => None
-    end.
-  Arguments fmap_maybe [A B] f ma.
-  Hint Unfold fmap_maybe : soundness.
-
-  Lemma fmap_maybe_id {A} : (fmap_maybe (B:=A)) id = id.
-  Proof. 
-    unfold fmap_maybe. ext. destruct x; reflexivity.
-  Qed.
-
-  Lemma fmap_maybe_compose : ∀ {A B C} (f : A → B) (g : B → C),
-    fmap_maybe (f ∘ g) = fmap_maybe f ∘ fmap_maybe g.
-  Proof. simple_solve. Qed.
-  Arguments fmap_maybe_compose [A B C] f g.
-
-  Global Instance functor_maybe : Functor (Maybe) := 
-  {
-    fmap := fmap_maybe;
-    fmap_id := @fmap_maybe_id;
-    fmap_compose := fmap_maybe_compose;
-  }.
-End Maybe_Functor.
-Hint Unfold fmap_maybe : soundness.
-Hint Rewrite @fmap_maybe_id @fmap_maybe_compose : soundness.
-
-Section Maybe_Applicative.
-  Definition app_maybe {A B} 
-    (Mf : Maybe (A -> B)) (Ma : Maybe A) : Maybe B :=
-    match Mf, Ma with
-    | None, _ => None
-    | _, None => None
-    | Just f, Just x => Just (f x)
-    end.
-  Arguments app_maybe [A B] Mf Ma.
-  Hint Unfold app_maybe : soundness.
-
-  Lemma app_maybe_id : 
-    ∀ {A} (f : Maybe A), app_maybe (Just id) f = f.
-  Proof. simple_solve. Qed.
-  Arguments app_maybe_id [A].
-
-  Lemma app_maybe_homomorphism :
-    ∀ {A B} (f : A → B) (x : A), 
-    app_maybe (Just f) (Just x) = Just (f x).
-  Proof. simple_solve. Qed.
-  Arguments app_maybe_homomorphism [A B] f x.
-
-  Lemma app_maybe_interchange :
-    ∀ {A B} (u : Maybe (A → B)) (y : A),
-    app_maybe u (Just y) = app_maybe (Just (λ f : A → B, f y)) u.
-  Proof. simple_solve. Qed.
-  Arguments app_maybe_interchange [A B] u y.
-
-  Lemma app_maybe_compose :
-    ∀ {A B C} (u : Maybe (B → C)) (v : Maybe (A → B)) (w : Maybe A),
-    app_maybe u (app_maybe v w) =
-    app_maybe (app_maybe (app_maybe (Just compose) u) v) w.
-  Proof. simple_solve. Qed.
-  Arguments app_maybe_compose [A B C] u v w.
-
-  Lemma app_maybe_fmap : ∀ {A B} (f : A → B) (x : Maybe A), 
-    fmap f x = app_maybe (Just f) x.
-  Proof. simple_solve. Qed.
-  Arguments app_maybe_fmap [A B] f x.
-
-  Lemma just_inj : ∀ (A : Type) (x y : A), Just x = Just y → x = y.
-  Proof.
-    intros A x y Heq. inv Heq. reflexivity.
-  Qed.
-
-  Global Instance applicative_maybe : Applicative Maybe :=
-  {
-    pure := @Just;
-    pure_inj := just_inj;
-    app := app_maybe;
-    app_id := app_maybe_id;
-    app_homomorphism := app_maybe_homomorphism;
-    app_interchange := app_maybe_interchange;
-    app_compose := app_maybe_compose;
-    app_fmap := app_maybe_fmap;
-  }. 
-End Maybe_Applicative.
-Hint Unfold app_maybe : soundness.
-Hint Rewrite @app_maybe_id @app_maybe_homomorphism : soundness.
 
 Section Maybe_Monad.
   Definition bind_maybe {A B} 
@@ -131,33 +40,18 @@ Section Maybe_Monad.
   Proof. simple_solve. Qed.
   Arguments bind_maybe_assoc [A B C] MA f g.
 
-  Lemma bind_maybe_app : ∀ {A B} (mf : Maybe (A → B)) (ma : Maybe A),
-    mf <*> ma =
-  bind_maybe mf (λ f : A → B, bind_maybe ma (λ a : A, (f ∘ pure) a)).
-  Proof. simple_solve. Qed.
-  Arguments bind_maybe_app [A B] mf ma.
-
-  Lemma bind_maybe_fmap : ∀ {A B C} (f : A → B) (x : Maybe A) (g : B → Maybe C),
-    bind_maybe (f <$> x) g = bind_maybe x (f ∘ g).
+  Lemma just_inj : ∀ A (x y : A),
+    Just x = Just y → x = y.
   Proof. 
-    intros. unfold bind_maybe. unfold compose. destruct x; reflexivity.
+    intros A x y Heq. inversion Heq. reflexivity.
   Qed.
-  Arguments bind_maybe_fmap [A B C] f x g.
-
-  Lemma bind_maybe_pass : ∀ {A B : Type} (ma : Maybe A) (mb : Maybe B),
-    ma >> mb = bind_maybe ma (λ _ : A, mb).
-  Proof. simple_solve. Qed.
-  Arguments bind_maybe_pass [A B] ma mb.
 
   Global Instance monad_maybe : Monad Maybe :=
   {
-    bindM := bind_maybe;
+    returnM_inj := just_inj;
     bind_id_left := bind_maybe_id_left;
     bind_id_right := bind_maybe_id_right;
     bind_assoc := bind_maybe_assoc;
-    bind_app := bind_maybe_app;
-    bind_fmap := bind_maybe_fmap;
-    bind_pass := bind_maybe_pass;
   }. 
 End Maybe_Monad.
 Hint Rewrite @bind_maybe_id_left @bind_maybe_id_right : soundness.
@@ -169,107 +63,6 @@ Inductive AbstractMaybe (A : Type) : Type :=
 Arguments JustA {_}.
 Arguments JustOrNoneA {_}.
 Arguments NoneA {_}.
-
-Section AbstractMaybe_Functor.
-  Definition fmap_abstract_maybe {A B : Type} 
-    (f : A -> B) (ma : AbstractMaybe A) : AbstractMaybe B :=
-    match ma with
-    | JustA a => JustA (f a)
-    | JustOrNoneA a => JustOrNoneA (f a)
-    | NoneA => NoneA
-    end. 
-  Arguments fmap_abstract_maybe [_ _] _ _.
-  Hint Unfold fmap_abstract_maybe : soundness.
-
-  Lemma fmap_abstract_maybe_id : ∀ {A}, fmap_abstract_maybe (@id A) = id.
-  Proof. simple_solve. Qed.
-  Arguments fmap_abstract_maybe_id {A}.
-
-  Lemma fmap_abstract_maybe_compose : ∀ {A B C : Type} (f : A → B) (g : B → C),
-  fmap_abstract_maybe (f ∘ g) = fmap_abstract_maybe f ∘ fmap_abstract_maybe g.
-  Proof. simple_solve. Qed.
-  Arguments fmap_abstract_maybe_compose [A B C] f g.
-
-  Global Instance functor_abstract_maybe : Functor AbstractMaybe :=
-  {
-    fmap := fmap_abstract_maybe;
-    fmap_id := @fmap_abstract_maybe_id;
-    fmap_compose := fmap_abstract_maybe_compose;
-  }.
-End AbstractMaybe_Functor.
-Hint Unfold fmap_abstract_maybe : soundness.
-Hint Rewrite @fmap_abstract_maybe_id @fmap_abstract_maybe_compose : soundness.
-
-Section AbstractMaybe_Applicative.
-  Definition app_abstract_maybe {A B : Type} (Mf : AbstractMaybe (A -> B))
-    (Ma : AbstractMaybe A) : AbstractMaybe B :=
-  match Mf, Ma with
-  | NoneA, _ => NoneA
-  | _, NoneA => NoneA
-  | JustOrNoneA f, JustOrNoneA a
-  | JustOrNoneA f, JustA a 
-  | JustA f, JustOrNoneA a => JustOrNoneA (f a)
-  | JustA f, JustA a => JustA (f a)
-  end.
-  Arguments app_abstract_maybe [_ _] _ _.
-  Hint Unfold app_abstract_maybe : soundness.
-
-  Lemma app_abstract_maybe_id : ∀ {A} (f : AbstractMaybe A),
-    app_abstract_maybe (JustA id) f = f.
-  Proof. simple_solve. Qed.
-  Arguments app_abstract_maybe_id [A].
-
-  Lemma app_abstract_maybe_homomorphism : ∀ {A B} (f : A → B) (x : A),
-  app_abstract_maybe (JustA f) (JustA x) = JustA (f x).
-  Proof. simple_solve. Qed.
-  Arguments app_abstract_maybe_homomorphism [A B] f x.
-
-  Lemma app_abstract_maybe_interchange : ∀ {A B}
-    (u : AbstractMaybe (A → B)) (y : A),
-    app_abstract_maybe u (JustA y) =
-    app_abstract_maybe (JustA (λ f : A → B, f y)) u.
-  Proof. simple_solve. Qed.
-  Arguments app_abstract_maybe_interchange [A B] u y.
-
-  Lemma app_abstract_maybe_compose : ∀ {A B C} 
-    (u : AbstractMaybe (B → C)) (v : AbstractMaybe (A → B)) 
-    (w : AbstractMaybe A),
-    app_abstract_maybe u (app_abstract_maybe v w) =
-    app_abstract_maybe
-      (app_abstract_maybe (app_abstract_maybe (JustA compose) u) v) w.
-  Proof. simple_solve. Qed.
-  Arguments app_abstract_maybe_compose [A B C] u v w.
-
-  Lemma app_abstract_maybe_fmap : ∀ {A B} (f : A → B) 
-    (x : AbstractMaybe A),
-  fmap f x = app_abstract_maybe (JustA f) x.
-  Proof. simple_solve. Qed.
-  Arguments app_abstract_maybe_fmap [A B] f x.
-
-  Lemma justA_inj : ∀ (A : Type) (x y : A), JustA x = JustA y → x = y.
-  Proof.
-    intros A x y Heq. inv Heq. reflexivity.
-  Qed.
-
-  Lemma justOrNoneA_inj : ∀ (A : Type) (x y : A),
-    JustOrNoneA x = JustOrNoneA y → x = y.
-  Proof.
-    intros A x y Heq. inv Heq. reflexivity.
-  Qed.
-
-  Global Instance applicative_abstract_maybe : Applicative AbstractMaybe :=
-  {
-    pure := @JustA;
-    pure_inj := justA_inj;
-    app := app_abstract_maybe;
-    app_id := app_abstract_maybe_id;
-    app_homomorphism := app_abstract_maybe_homomorphism; 
-    app_interchange := app_abstract_maybe_interchange;
-    app_compose := app_abstract_maybe_compose;
-    app_fmap := app_abstract_maybe_fmap;
-  }.
-End AbstractMaybe_Applicative.
-Hint Resolve @app_abstract_maybe_id @app_abstract_maybe_homomorphism : soundness.
 
 Section AbstractMaybe_Monad.
   Definition bind_maybeA {A B : Type}
@@ -303,190 +96,34 @@ Section AbstractMaybe_Monad.
   Proof. solve_monad. Qed.
   Arguments bind_maybeA_assoc [A B C] MA f g.
 
-  Lemma bind_maybeA_fmap : ∀ {A B C} (f : A → B) 
-    (x : AbstractMaybe A) (g : B → AbstractMaybe C),
-    bind_maybeA (f <$> x) g = bind_maybeA x (f ∘ g).
-  Proof. 
-    destruct x; reflexivity.
+  Lemma justA_inj : ∀ A (x y : A),
+    JustA x = JustA y → x = y.
+  Proof.
+    intros A x y Heq. inversion Heq. reflexivity.
   Qed.
-  Arguments bind_maybeA_fmap [A B C] f x.
-
-  Lemma bind_maybeA_app : ∀ {A B} (mf : AbstractMaybe (A → B)) 
-    (ma : AbstractMaybe A),
-    app_abstract_maybe mf ma =
-    bind_maybeA mf (λ f : A → B, bind_maybeA ma (λ a : A, (f ∘ pure) a)).
-  Proof. destruct mf, ma; reflexivity. Qed.
-  Arguments bind_maybeA_app [A B] mf ma.
-
-  Lemma bind_maybeA_pass : ∀ {A B} (ma : AbstractMaybe A) 
-    (mb : AbstractMaybe B),
-    ma >> mb = bind_maybeA ma (λ _ : A, mb).
-  Proof. destruct ma, mb; reflexivity. Qed.
-  Arguments bind_maybeA_pass [A B] ma mb.
 
   Global Instance monad_abstract_maybe : Monad AbstractMaybe :=
   {
+    returnM_inj := justA_inj;
     bindM := bind_maybeA;
     bind_id_left := bind_maybeA_id_left;
     bind_id_right := bind_maybeA_id_right;
     bind_assoc := bind_maybeA_assoc;
-    bind_fmap := bind_maybeA_fmap;
-    bind_app := bind_maybeA_app;
-    bind_pass := bind_maybeA_pass;
   }. 
 End AbstractMaybe_Monad.
 Hint Rewrite @bind_maybeA_id_left @bind_maybeA_id_right : soundness.
 
 Definition MaybeT M A: Type := M (Maybe A).
 
-Section MaybeT_Functor.
-  Context {M} `{M_monad : Monad M}.
-
-  Definition fmap_maybeT {A B} (f : A -> B)
-    (m : MaybeT M A) : MaybeT M B :=  fmap (fmap (M:=Maybe) f) m. 
-  Arguments fmap_maybeT [_ _] _ _.
-  Hint Unfold fmap_maybeT : soundness.
-
-  Lemma fmap_maybeT_id : ∀ {A}, fmap_maybeT (@id A) = id.
-  Proof. simple_solve. Qed.
-
-  Lemma fmap_maybeT_compose : ∀ {A B C} (f : A → B) (g : B → C),
-  fmap_maybeT (f ∘ g) = fmap_maybeT f ∘ fmap_maybeT g.
-  Proof. 
-    intros. unfold fmap_maybeT. ext.
-    repeat rewrite fmap_compose. 
-    reflexivity.
-  Qed.
-  Arguments fmap_maybeT_compose [A B C] f g.
-
-  Global Instance functor_maybeT : Functor (MaybeT M) :=
-  {
-    fmap := fmap_maybeT;
-    fmap_id := @fmap_maybeT_id;
-    fmap_compose := fmap_maybeT_compose;
-  }.
-End MaybeT_Functor.
-Hint Unfold fmap_maybeT : soundness.
-Hint Rewrite @fmap_maybeT_id @fmap_maybeT_compose : soundness.
-
-Section MaybeT_Applicative.
-  Context {M} `{M_monad : Monad M}.
-
-  Definition pure_maybeT {A} (x : A) : MaybeT M A :=
-    pure (Just x).
-  Arguments pure_maybeT [_] _.
-  Hint Unfold pure_maybeT : soundness.
-
-  Definition app_maybeT {A B} (Mmf : MaybeT M (A -> B))
-    (Mma : MaybeT M A) : MaybeT M B := 
-    bindM (M:=M) (A:=(Maybe (A → B))) Mmf (λ mf : Maybe (A → B),
-      match mf with
-      | Just f =>
-          bindM (M:=M) (A:=(Maybe A)) Mma (λ m,
-            match m with
-            | Just a => pure (M:=M) (Just (f a))
-            | None => pure (M:=M) None
-            end)
-      | None => pure None
-      end).
-  Arguments app_maybeT [A B] Mmf Mma.
-  Hint Unfold app_maybeT : soundness.
-
-  Lemma app_maybeT_id : ∀ {A} (f : MaybeT M A),
-    app_maybeT (pure_maybeT id) f = f.
-  Proof. 
-    intros. unfold app_maybeT, pure_maybeT.
-    autorewrite with soundness.
-    rewrite <- (bind_id_right (M:=M)). 
-    f_equal; ext. destruct x; reflexivity.
-  Qed.
-  Arguments app_maybeT_id [A] f.
-
-  Lemma app_maybeT_homomorphism : ∀ {A B} (f : A → B) (x : A),
-  app_maybeT (pure_maybeT f) (pure_maybeT x) = pure_maybeT (f x).
-  Proof. solve_monad. Qed.
-  Arguments app_maybeT_homomorphism [A B] f x.
-
-  Lemma app_maybeT_interchange : ∀ {A B} (u : MaybeT M (A → B)) (y : A),
-  app_maybeT u (pure_maybeT y) = app_maybeT (pure_maybeT (λ f : A → B, f y)) u.
-  Proof. 
-    intros. unfold app_maybeT, pure_maybeT.
-    autorewrite with soundness. f_equal. ext. 
-    destruct x; autorewrite with soundness; reflexivity.
-  Qed.
-  Arguments app_maybeT_interchange [A B] u y.
-
-  Lemma app_maybeT_compose : ∀ {A B C} (u : MaybeT M (B → C)) 
-    (v : MaybeT M (A → B))  (w : MaybeT M A),
-    app_maybeT u (app_maybeT v w) =
-    app_maybeT (app_maybeT (app_maybeT (pure_maybeT compose) u) v) w.
-  Proof. 
-    intros. unfold app_maybeT, pure_maybeT. rewrite bind_id_left.
-    repeat rewrite bind_assoc. f_equal; ext. destruct x. rewrite bind_id_left.
-    repeat rewrite bind_assoc. f_equal; ext. destruct x. rewrite bind_id_left.
-    repeat rewrite bind_assoc. f_equal; ext. destruct x. rewrite bind_id_left.
-    reflexivity. rewrite bind_id_left. reflexivity. repeat rewrite bind_id_left.
-    reflexivity. repeat rewrite bind_id_left. reflexivity.
-  Qed.
-  Arguments app_maybeT_compose [A B C] u v w.
-
-  Lemma fmap_app_maybeT : ∀ {A B} (f : A → B) (x : MaybeT M A),
-  fmap_maybeT f x = app_maybeT (pure_maybeT f) x.
-  Proof. 
-    intros. unfold fmap_maybeT, app_maybeT, pure_maybeT.
-    rewrite bind_id_left. simpl. unfold fmap_maybe.
-    rewrite fmap_bind_pure. f_equal. ext. destruct x0; reflexivity.
-  Qed.
-  Arguments fmap_app_maybeT [A B] f x.
-
-  Lemma pure_maybeT_inj : ∀ (A : Type) (x y : A),
-    pure_maybeT x = pure_maybeT y → x = y.
-  Proof.
-    intros. apply just_inj, pure_inj. easy.
-  Qed.
-
-  Global Instance applicative_maybeT : Applicative (MaybeT M) :=
-  {
-    pure := pure_maybeT;
-    pure_inj := pure_maybeT_inj;
-    app := app_maybeT;
-    app_id := app_maybeT_id;
-    app_homomorphism := app_maybeT_homomorphism;
-    app_interchange := app_maybeT_interchange;
-    app_compose := app_maybeT_compose;
-    app_fmap := fmap_app_maybeT;
-  }. 
-End MaybeT_Applicative.
-Hint Unfold pure_maybeT app_maybeT : soundness.
-Hint Rewrite @app_maybeT_id @app_maybeT_homomorphism : soundness.
-Definition NoneT {M A} `{M_monad : Monad M} : MaybeT M A := pure None.
-Hint Unfold NoneT : soundness.
-Definition JustT {M A} `{M_monad : Monad M} (a : A) : MaybeT M A := pure (Just a).
-Hint Unfold JustT : soundness.
-
-Section maybeT_laws.
-  Context {M} `{M_monad : Monad M}.
-  Context {A}.
-
-  Lemma justT_eq_noneT_false : ∀ x : A, JustT x ≠ NoneT.
-  Proof.
-    unfold not. intros. 
-    absurd (Just x = None). easy. 
-    apply pure_inj. easy. 
-  Qed.
-
-  Lemma justT_inj : ∀ x y: A, JustT x = JustT y → x = y.
-  Proof.
-    intros. apply just_inj, pure_inj. assumption.
-  Qed.
-End maybeT_laws.
-
 Section MaybeT_Monad.
   Context {M} `{M_monad : Monad M}.
 
-  Definition bind_maybeT {A B} (x : MaybeT M A)
+  Definition NoneT {A} : MaybeT M A := returnM None.
+  Definition JustT {A} (a : A) : MaybeT M A := returnM (Just a).
+
+  Definition bind_maybeT {A B} (x : MaybeT M A) 
     (f : A -> MaybeT M B) : MaybeT M B :=
-    @bindM M _ _ _ (Maybe A) (Maybe B) x (λ v,
+    bindM (M:=M) x (λ v : Maybe A,
       match v with
       | None => NoneT
       | Just a => f a
@@ -496,20 +133,20 @@ Section MaybeT_Monad.
   Hint Unfold bind_maybeT : soundness.
 
   Lemma bind_maybeT_id_left : ∀ {A B} (f : A → MaybeT M B) (a : A), 
-    bind_maybeT (pure a) f = f a.
+    bind_maybeT (JustT a) f = f a.
   Proof. 
-    intros. unfold bind_maybeT. unfold pure. simpl. unfold pure_maybeT.
+    intros. unfold bind_maybeT, JustT. 
     rewrite bind_id_left. reflexivity.
   Qed.
   Arguments bind_maybeT_id_left [A B] f a.
 
   Lemma bind_maybeT_id_right : ∀ {A} (MA : MaybeT M A),
-    bind_maybeT MA pure = MA.
+    bind_maybeT MA JustT = MA.
   Proof. 
-    intros. unfold bind_maybeT. 
-    replace (MA) with (bindM (M:=M) MA pure) at 2.
+    intros. unfold bind_maybeT, NoneT, JustT. 
+    replace (MA) with (bindM (M:=M) MA returnM) at 2.
     f_equal. ext; destruct x; reflexivity.
-    rewrite <- (bind_id_right (M:=M)). f_equal. 
+    rewrite <- (bind_id_right (M:=M)). reflexivity.
   Qed.
   Arguments bind_maybeT_id_right [A] MA.
 
@@ -524,50 +161,22 @@ Section MaybeT_Monad.
   Qed.
   Arguments bind_maybeT_assoc [A B C] MA f g.
 
-  Lemma bind_maybeT_app : ∀ {A B} (mf : MaybeT M (A → B)) 
-    (ma : MaybeT M A),
-    mf <*> ma = 
-    bind_maybeT mf (λ f : A → B, bind_maybeT ma (λ a : A, (f ∘ pure) a)).
-  Proof. simple_solve. Qed.
-  Arguments bind_maybeT_app [A B] mf ma.
-
-  Lemma bind_maybeT_fmap : ∀ {A B C} (f : A → B) 
-    (x : MaybeT M A) (g : B → MaybeT M C),
-    bind_maybeT (fmap f x) g = bind_maybeT x (f ∘ g).
-  Proof. 
-    intros. unfold bind_maybeT. unfold fmap; simpl. unfold fmap_maybeT.
-    rewrite bind_fmap. f_equal. ext. unfold compose. 
-    destruct x0; reflexivity.
+  Lemma justT_inj : ∀ A (x y : A),
+    JustT x = JustT y → x = y.
+  Proof.
+    intros. apply just_inj, returnM_inj. assumption.
   Qed.
-  Arguments bind_maybeT_fmap [A B C] f x g.
-
-  Lemma bind_maybeT_pass : ∀ {A B} (ma : MaybeT M A) (mb : MaybeT M B),
-    ma >> mb = bind_maybeT ma (λ _ : A, mb).
-  Proof. 
-    intros. unfold bind_maybeT. simpl.
-    unfold app_maybeT, fmap_maybeT. autorewrite with soundness.
-    f_equal. ext. unfold compose. autorewrite with soundness.
-    destruct x; simpl. rewrite <- bind_id_right. f_equal.
-    ext. destruct x; autorewrite with soundness. unfold const.
-    autorewrite with soundness. all:reflexivity.
-  Qed.
-  Arguments bind_maybeT_pass [A B] ma mb.
 
   Global Instance monad_maybeT : Monad (MaybeT M) :=
   {
-    bindM := bind_maybeT;
+    returnM_inj := justT_inj;
     bind_id_left := bind_maybeT_id_left;
     bind_id_right := bind_maybeT_id_right;
     bind_assoc := bind_maybeT_assoc;
-    bind_app := bind_maybeT_app;
-    bind_fmap := bind_maybeT_fmap;
-    bind_pass := bind_maybeT_pass;
   }. 
 End MaybeT_Monad.
 Hint Unfold bind_maybeT : soundness.
-Hint Rewrite @bind_maybeT_id_left 
-             @bind_maybeT_id_right 
-             @bind_maybeT_app @bind_maybeT_fmap : soundness.
+Hint Rewrite @bind_maybeT_id_left @bind_maybeT_id_right : soundness.
 
 Section MaybeT_MonadT.
   Context {M} `{M_monad : Monad M}.
@@ -576,10 +185,9 @@ Section MaybeT_MonadT.
     bindM (M:=M) Ma (λ a, JustT a).
   Arguments lift_maybeT [_] _.
   Hint Unfold lift_maybeT : soundness.
-  Hint Rewrite @fmap_bind @bind_fmap : soundness.
 
   Lemma lift_maybeT_pure : ∀ (A : Type) (x : A),
-    lift_maybeT (pure x) = pure x.
+    lift_maybeT (returnM x) = returnM x.
   Proof. solve_monad. Qed.
 
   Lemma lift_maybeT_bind : ∀ (A B : Type) (x : M A) (f : A → M B),
@@ -592,223 +200,51 @@ Section MaybeT_MonadT.
 
   Global Instance monadT_maybeT : MonadT (MaybeT) :=
   {
-    liftT := lift_maybeT;
-    lift_pure := lift_maybeT_pure;
+    lift_return := lift_maybeT_pure;
     lift_bind := lift_maybeT_bind;
   }. 
 End MaybeT_MonadT.
 
 Definition MaybeAT M A : Type := M (AbstractMaybe A).
 
-Section MaybeAT_Functor.
-  Context {M} `{M_functor : Functor M}.
-
-  Definition fmap_maybeAT {A B} 
-    (f : A -> B) (Ma : MaybeAT M A) : MaybeAT M B :=
-    fmap (fmap_abstract_maybe f) Ma.
-  Arguments fmap_maybeAT [A B] f Ma.
-  Hint Unfold fmap_maybeAT : soundness.
-
-  Lemma fmap_maybeAT_id : ∀ A, fmap_maybeAT (@id A) = id.
-  Proof.
-    unfold fmap_maybeAT. intros. ext. autorewrite with soundness.
-    reflexivity.
-  Qed.
-
-  Lemma fmap_maybeAT_compose : ∀ (A B C : Type) (f : A → B) (g : B → C),
-    fmap_maybeAT (f ∘ g) = fmap_maybeAT f ∘ fmap_maybeAT g.
-  Proof.
-    intros. unfold fmap_maybeAT. ext. autorewrite with soundness. reflexivity.
-  Qed.
-
-  Global Instance functor_maybeAT : Functor (MaybeAT M) :=
-  {
-    fmap := fmap_maybeAT;
-    fmap_id := fmap_maybeAT_id;
-    fmap_compose := fmap_maybeAT_compose;
-  }. 
-End MaybeAT_Functor.
-Hint Unfold fmap_maybeAT : soundness.
-
-Section MaybeAT_Applicative.
-  Context {M} `{M_monad : Monad M}.
-
-  Definition pure_maybeAT {A} (x : A) : MaybeAT M A :=
-    pure (JustA x).
-  Arguments pure_maybeAT [A] x.
-  Hint Unfold pure_maybeAT : soundness.
-
-  Definition app_maybeAT {A B} (Mmf : MaybeAT M (A -> B))
-    (Mma : MaybeAT M A) : MaybeAT M B :=
-    @bindM M _ _ _ _ _ Mmf 
-      (λ mf : AbstractMaybe (A -> B),
-      match mf with 
-      | JustA f => @bindM M _ _ _ _ _ Mma 
-          (λ ma : AbstractMaybe A,
-          match ma with
-          | JustOrNoneA a => pure (JustOrNoneA (f a))
-          | JustA a => pure (JustA (f a))
-          | NoneA => pure NoneA
-          end)
-      | JustOrNoneA f => @bindM M _ _ _ _ _ Mma (λ ma : AbstractMaybe A,
-          match ma with
-          | JustA a | JustOrNoneA a => pure (JustOrNoneA (f a))
-          | NoneA => pure NoneA
-          end)
-      | NoneA => pure NoneA
-      end).
-  Arguments app_maybeAT [A B] Mmf Mma.
-  Hint Unfold app_maybeAT : soundness.
-
-  Lemma app_maybeAT_id : ∀ {A} (f : MaybeAT M A), 
-    app_maybeAT (pure_maybeAT id) f = f.
-  Proof. 
-    intros. unfold app_maybeAT, pure_maybeAT. autorewrite with soundness.
-    rewrite <- (bind_id_right (M:=M)). f_equal; ext. 
-    destruct_all (AbstractMaybe A); reflexivity.
-  Qed.
-  Arguments app_maybeAT_id [A] f.
-
-  Lemma app_maybeAT_homomorphism : ∀ {A B} (f : A → B) (x : A),
-    app_maybeAT (pure_maybeAT f) (pure_maybeAT x) = pure_maybeAT (f x).
-  Proof. 
-    intros. unfold app_maybeAT, pure_maybeAT. autorewrite with soundness.
-    reflexivity.
-  Qed.
-  Arguments app_maybeAT_homomorphism [A B] f x.
-
-  Lemma app_maybeAT_interchange : ∀ {A B} (u : MaybeAT M (A → B)) (y : A),
-    app_maybeAT u (pure_maybeAT y) = 
-    app_maybeAT (pure_maybeAT (λ f : A → B, f y)) u.
-  Proof. 
-    intros. unfold app_maybeAT, pure_maybeAT. autorewrite with soundness.
-    f_equal. ext. destruct x; autorewrite with soundness; reflexivity.
-  Qed.
-  Arguments app_maybeAT_interchange [A B] u y.
-
-  Lemma app_maybeAT_compose : ∀ {A B C}
-    (u : MaybeAT M (B → C)) (v : MaybeAT M (A → B)) (w : MaybeAT M A),
-    app_maybeAT u (app_maybeAT v w) =
-    app_maybeAT (app_maybeAT (app_maybeAT (pure_maybeAT compose) u) v) w.
-  Proof. 
-    intros; unfold app_maybeAT, pure_maybeAT; rewrite bind_id_left;
-    repeat rewrite bind_assoc; f_equal; ext; destruct x; 
-    repeat rewrite bind_id_left; try reflexivity;
-    repeat rewrite bind_assoc; f_equal; ext; destruct x;
-    repeat rewrite bind_id_left; try reflexivity;
-    repeat rewrite bind_assoc; f_equal; ext; destruct x;
-    repeat rewrite bind_id_left; reflexivity.
-  Qed.
-  Hint Unfold fmap_maybeAT : soundness.
-  Arguments app_maybeAT_compose [A B C] u v w.
-
-  Lemma app_maybeAT_fmap : ∀ {A B} (f : A → B) (x : MaybeAT M A),
-    f <$> x = app_maybeAT (pure_maybeAT f) x.
-  Proof.
-    intros. unfold app_maybeAT, pure_maybeAT. rewrite bind_id_left.
-    unfold fmap; simpl. unfold fmap_maybeAT.
-    unfold fmap_abstract_maybe. rewrite fmap_bind_pure.
-    f_equal; ext. unfold compose. destruct x0; reflexivity.
-  Qed.
-  Arguments app_maybeAT_fmap [A B] f x.
-
-  Lemma pure_maybeAT_inj : ∀ (A : Type) (x y : A),
-    pure_maybeAT x = pure_maybeAT y → x = y.
-  Proof.
-    intros. apply justA_inj, pure_inj; auto.
-  Qed.
-
-  Global Instance applicative_maybeAT : Applicative (MaybeAT M) :=
-  {
-    pure := pure_maybeAT;
-    pure_inj := pure_maybeAT_inj;
-    app := app_maybeAT;
-    app_id := app_maybeAT_id;
-    app_homomorphism := app_maybeAT_homomorphism;
-    app_interchange := app_maybeAT_interchange;
-    app_compose := app_maybeAT_compose;
-    app_fmap := app_maybeAT_fmap;
-  }. 
-End MaybeAT_Applicative.
-Hint Unfold pure_maybeAT app_maybeAT : soundness.
-
-Definition NoneAT {M A} `{M_monad : Monad M} : MaybeAT M A := pure NoneA.
-Hint Unfold NoneAT : soundness.
-Definition JustAT {M A} `{M_monad : Monad M} (a : A) : MaybeAT M A := pure (JustA a).
-Hint Unfold JustAT : soundness.
-Definition JustOrNoneAT {M A} `{M_monad : Monad M} (a : A) : MaybeAT M A := 
-  pure (JustOrNoneA a).
-Hint Unfold JustOrNoneAT : soundness.
-
-Section MaybeAT_laws.
-  Context {M : Type → Type} `{M_monad : Monad M}.
-  Context {A}.
-
-  Lemma noneAT_neq_justAT : ∀ (a : A), NoneAT ≠ JustAT a.
-  Proof.
-    intros. unfold not; intro. absurd (NoneA = JustA a). easy.
-    apply pure_inj; easy.
-  Qed.
-
-  Lemma noneAT_neq_justornoneAT : ∀ (a : A), NoneAT ≠ JustOrNoneAT a.
-  Proof.
-    intros. unfold not. intros. absurd (NoneA = JustOrNoneA a). easy.
-    apply pure_inj; easy.
-  Qed.
-
-  Lemma justAT_neq_justornoneAT : ∀ (a a' : A), 
-    JustAT a ≠ JustOrNoneAT a'.
-  Proof.
-    intros. unfold not. intros. absurd (JustA a = JustOrNoneA a'). easy.
-    apply pure_inj. easy.
-  Qed.
-
-  Lemma justAT_inj : ∀ (x y : A), JustAT x = JustAT y → x = y.
-  Proof.
-    intros. apply justA_inj, pure_inj; easy.
-  Qed.
-
-  Lemma justOrNoneAT_inj : ∀ (x y : A),
-    JustOrNoneAT x = JustOrNoneAT y → x = y.
-  Proof.
-    intros. apply justOrNoneA_inj, pure_inj. easy.
-  Qed.
-End MaybeAT_laws.
-
 Section MaybeAT_Monad.
   Context {M} `{M_monad : Monad M}.
+
+  Definition NoneAT {A} : MaybeAT M A := returnM NoneA.
+  Definition JustAT {A} (a : A) : MaybeAT M A := returnM (JustA a).
+  Definition JustOrNoneAT {A} (a : A) : MaybeAT M A := 
+    returnM (JustOrNoneA a).
 
   Definition bind_maybeAT {A B} 
     (Mma : MaybeAT M A)
     (f : A -> MaybeAT M B) : MaybeAT M B :=
-  @bindM M _ _ _ (AbstractMaybe A) (AbstractMaybe B) Mma (fun ma =>
+  @bindM M _ (AbstractMaybe A) (AbstractMaybe B) Mma (fun ma =>
     match ma with
-    | NoneA => pure NoneA
+    | NoneA => returnM NoneA
     | JustA a => f a
     | JustOrNoneA a => 
-        @bindM M _ _ _ (AbstractMaybe B) (AbstractMaybe B) (f a) (fun mfa =>
+        @bindM M _ (AbstractMaybe B) (AbstractMaybe B) (f a) (fun mfa =>
                        match mfa with
-                       | NoneA => pure NoneA
-                       | JustA b => pure (JustOrNoneA b)
-                       | JustOrNoneA b => pure (JustOrNoneA b)
+                       | NoneA => returnM NoneA
+                       | JustA b => returnM (JustOrNoneA b)
+                       | JustOrNoneA b => returnM (JustOrNoneA b)
                        end)
     end).
   Hint Unfold bind_maybeAT : soundness.
 
   Lemma bind_maybeAT_id_left : ∀ {A B} (f : A → MaybeAT M B) (a : A), 
-    bind_maybeAT (pure_maybeAT a) f = f a.
+    bind_maybeAT (JustAT a) f = f a.
   Proof. 
-    unfold pure; simpl. intros. unfold bind_maybeAT, pure_maybeAT. 
+    unfold JustAT, bind_maybeAT; simpl. intros.
     rewrite bind_id_left. reflexivity.
   Qed.
   Arguments bind_maybeAT_id_left [A B] f a.
 
   Lemma bind_maybeAT_id_right : ∀ {A} (MA : MaybeAT M A), 
-    bind_maybeAT MA pure_maybeAT = MA.
+    bind_maybeAT MA JustAT = MA.
   Proof. 
-    unfold bind_maybeAT. intros. rewrite <- (bind_id_right (M:=M)).
-    f_equal; extensionality x. destruct x; unfold pure_maybeAT. reflexivity.
-    autorewrite with soundness. reflexivity. reflexivity.
+    unfold bind_maybeAT, JustAT. intros. rewrite <- (bind_id_right (M:=M)).
+    f_equal; extensionality x. destruct x; autorewrite with soundness; reflexivity.
   Qed.
   Arguments bind_maybeAT_id_right [A] MA.
 
@@ -828,54 +264,19 @@ Section MaybeAT_Monad.
   Qed.
   Arguments bind_maybeAT_assoc [A B C] MA f g.
 
-  Lemma bind_maybeAT_app : ∀ {A B} (mf : MaybeAT M (A → B)) 
-    (ma : MaybeAT M A), app_maybeAT mf ma =
-    bind_maybeAT mf (λ f : A → B, bind_maybeAT ma (λ a : A, (f ∘ pure_maybeAT) a)).
+  Lemma justAT_inj : ∀ A (x y : A),
+    JustAT x = JustAT y → x = y.
   Proof.
-    intros. unfold bind_maybeAT, app_maybeAT. autorewrite with soundness. 
-    f_equal; ext. destruct x; autorewrite with soundness. 
-    f_equal; ext. destruct x. unfold pure_maybeAT.
-    unfold compose. reflexivity. unfold pure_maybeAT, compose.
-    autorewrite with soundness. reflexivity. reflexivity.
-    f_equal; ext. destruct x. unfold compose, pure_maybeAT.
-    autorewrite with soundness. reflexivity. unfold compose, pure_maybeAT.
-    autorewrite with soundness. reflexivity. autorewrite with soundness.
-    reflexivity. reflexivity.
+    intros. apply justA_inj, returnM_inj. assumption.
   Qed.
-  Arguments bind_maybeAT_app [A B] mf ma.
-
-  Lemma bind_maybeAT_fmap : ∀ {A B C} (f : A → B) (x : MaybeAT M A) 
-    (g : B → MaybeAT M C), bind_maybeAT (f <$> x) g = bind_maybeAT x (f ∘ g).
-  Proof.
-    intros. unfold fmap; simpl; unfold fmap_maybeAT, bind_maybeAT.
-    autorewrite with soundness. f_equal; ext. destruct x0;
-    unfold compose; autorewrite with soundness; reflexivity.
-  Qed.
-  Arguments bind_maybeAT_fmap [A B C] f x g.
-
-  Lemma bind_maybeAT_pass : ∀ {A B} (ma : MaybeAT M A) 
-    (mb : MaybeAT M B), ma >> mb = bind_maybeAT ma (λ _ : A, mb).
-  Proof.
-    intros. unfold app; simpl; unfold app_maybeAT, bind_maybeAT, fmap_maybeAT.
-    unfold fmap_abstract_maybe. autorewrite with soundness.
-    f_equal; ext. unfold compose. 
-    autorewrite with soundness.
-    destruct x; autorewrite with soundness. rewrite <- bind_id_right.
-    f_equal; ext. destruct x; unfold const; autorewrite with soundness;
-    reflexivity. reflexivity. reflexivity.
-  Qed.
-  Arguments bind_maybeAT_pass [A B] ma mb.
 
   Global Instance monad_maybeAT 
   : Monad (MaybeAT M) :=
   {
-    bindM := @bind_maybeAT;
+    returnM_inj := justAT_inj;
     bind_id_left := bind_maybeAT_id_left;
     bind_id_right := bind_maybeAT_id_right;
     bind_assoc := bind_maybeAT_assoc;
-    bind_app := bind_maybeAT_app;
-    bind_fmap := bind_maybeAT_fmap;
-    bind_pass := bind_maybeAT_pass;
   }. 
 End MaybeAT_Monad.
 Hint Unfold bind_maybeAT : soundness.
@@ -889,7 +290,7 @@ Section MaybeAT_MonadT.
   Hint Unfold lift_maybeAT : soundness.
 
   Definition lift_maybeAT_pure : ∀ {A} (x : A),
-    lift_maybeAT (pure x) = pure x.
+    lift_maybeAT (returnM x) = returnM x.
   Proof.
     solve_monad.
   Qed.
@@ -906,101 +307,25 @@ Section MaybeAT_MonadT.
 
   Global Instance monadT_maybeAT : MonadT MaybeAT :=
   {
-    liftT := lift_maybeAT;
-    lift_pure := lift_maybeAT_pure;
+    lift_return := lift_maybeAT_pure;
     lift_bind := lift_maybeAT_bind;
   }. 
-    
 End MaybeAT_MonadT.
 
 Definition State (S A : Type) := S -> (A * S).
 
-Section State_Functor.
-
-  Definition fmap_state {S A B} 
-    (f : A -> B) (Fa : State S A) : State S B := 
-    fun st => let (x, s) := Fa st in (f x, s).
-  Arguments fmap_state [S A B] f Fa.
-  Hint Unfold fmap_state : soundness.
-
-  Lemma fmap_state_id {S} : ∀ A, fmap_state (S:=S) (@id A) = id.
-  Proof. simple_solve. Qed. 
-
-  Lemma fmap_state_compose {S} : ∀ (A B C : Type) (f : A → B) (g : B → C),
-    fmap_state (S:=S) (f ∘ g) = fmap_state (S:=S) f ∘ fmap_state (S:=S) g.
-  Proof. solve_monad. Qed.
-
-  Global Instance functor_state {S} : Functor (State S) :=
-  {
-    fmap := @fmap_state S;
-    fmap_id := @fmap_state_id S;
-    fmap_compose := @fmap_state_compose S;
-  }. 
-
-End State_Functor.
-Hint Unfold fmap_state : soundness.
-
-Section State_Applicative.
-  Context {S : Type}. 
-
-  Definition pure_state {A} (a : A) : State S A :=
-    fun st => (a, st).
-  Arguments pure_state [A] a.
-
-  Definition app_state {A B} 
-    (Mf : State S (A -> B)) (Ma : State S A) : State S B :=
-    fun st => let (f, st') := Mf st in 
-              let (a, st'') := Ma st' in (f a, st'').
-  Arguments app_state [A B] Mf Ma.
-  Hint Unfold pure_state app_state : soundness.
-
-  Definition pure_state_inj : ∀ (A : Type) (x y : A),
-    @pure_state A x = @pure_state A y → x = y.
-  Proof.
-    unfold pure_state. intros A x y [= Hfun_eq].
-    eapply equal_f in Hfun_eq.
-    inversion Hfun_eq. reflexivity. Unshelve.
-  Admitted.
-
-  Lemma app_state_id : ∀ (A : Type) (x : State S A),
-    app_state (B:=A) (pure_state (@id A)) x = x.
-  Proof. simple_solve. Qed.
-  
-  Lemma app_state_homomorphism : ∀ (A B : Type) (f : A → B) (x : A),
-    app_state (pure_state f) (pure_state x) = pure_state (f x).
-  Proof. simple_solve. Qed.
-
-  Lemma app_state_interchange : ∀ (A B : Type) (u : State S (A → B)) (y : A),
-  app_state u (pure_state y) = 
-  app_state (pure_state (λ f : A → B, f y)) u.
-  Proof. simple_solve. Qed.
-
-  Lemma app_state_compose : ∀ (A B C : Type) (u : State S (B → C)) 
-    (v : State S (A → B)) (w : State S A),
-    app_state u (app_state v w) =
-    app_state (app_state (app_state (pure_state compose) u) v) w.
-  Proof. simple_solve. Qed.
-
-  Lemma app_state_fmap : ∀ (A B : Type) (f : A → B) (x : State S A),
-    fmap_state f x = app_state (pure_state f) x.
-  Proof. simple_solve. Qed.
-
-  Global Instance applicative_state : Applicative (State S) :=
-  {
-    pure := pure_state;
-    pure_inj := pure_state_inj;
-    app := app_state;
-    app_id := app_state_id;
-    app_homomorphism := app_state_homomorphism;
-    app_interchange := app_state_interchange;
-    app_compose := app_state_compose;
-    app_fmap := app_state_fmap;
-  }. 
-End State_Applicative.
-Hint Unfold app_state : soundness.
-
 Section State_Monad.
   Context {S : Type}.
+
+  Definition return_state {A} (a :A) : State S A := 
+    λ st : S, (a, st).
+
+  Lemma return_state_inj : ∀ A (x y : A),
+    return_state x = return_state y → x = y.
+  Proof.
+    intros. unfold return_state in H. 
+  Admitted.
+
   Definition bind_state {A B} 
     (p : State S A) (k : A -> State S B) : State S B :=
     fun st => match (p st) with
@@ -1010,11 +335,11 @@ Section State_Monad.
   Hint Unfold bind_state : soundness.
 
   Lemma bind_state_id_left : ∀ (A B : Type) (f : A → State S B) (a : A),
-    bind_state (pure a) f = f a.
+    bind_state (return_state a) f = f a.
   Proof. simple_solve. Qed.
 
   Lemma bind_state_id_right : ∀ (A : Type) (MA : State S A),
-    bind_state MA pure = MA.
+    bind_state MA return_state = MA.
   Proof. simple_solve. Qed.
 
   Lemma bind_state_assoc : ∀ (A B C : Type) (MA : State S A) 
@@ -1023,157 +348,31 @@ Section State_Monad.
     bind_state MA (λ a : A, bind_state (f a) g).
   Proof. simple_solve. Qed.
   
-  Lemma bind_state_app : ∀ (A B : Type) (mf : State S (A → B)) (ma : State S A),
-    app_state mf ma = 
-    bind_state mf (λ f : A → B, bind_state ma (λ a : A, (f ∘ pure) a)).
-  Proof. solve_monad. Qed.
-
-  Lemma bind_state_fmap : ∀ (A B C : Type) (f : A → B) (x : State S A) 
-    (g : B → State S C),
-    bind_state (fmap_state f x) g = bind_state x (f ∘ g).
-  Proof. solve_monad. Qed.
-
-  Lemma bind_state_pass : ∀ (A B : Type) (ma : State S A) (mb : State S B),
-    ma >> mb = bind_state ma (λ _ : A, mb).
-  Proof. simple_solve. Qed.
-
   Global Instance monad_state : Monad (State S) :=
   {
-    bindM := bind_state;
+    returnM_inj := return_state_inj;
     bind_id_left := bind_state_id_left;
     bind_id_right := bind_state_id_right;
     bind_assoc := bind_state_assoc;
-    bind_app := bind_state_app;
-    bind_fmap := bind_state_fmap;
-    bind_pass := bind_state_pass;
   }. 
 End State_Monad.
 Hint Unfold bind_state : soundness.
 
 Definition StateT S M A : Type := S → M (A*S)%type.
 
-Section Functor_StateT.
-  Context {M} `{M_monad : Monad M}.
-
-  Definition fmap_stateT {S A B} (f : A -> B) (m : StateT S M A)
-    : StateT S M B :=
-    fun s : S => bindM (m s) 
-      (fun x => let (a, s') := x : (A*S)%type in pure (f a, s')).
-  Arguments fmap_stateT [S A B] f m.
-  Hint Unfold fmap_stateT : soundness.
-
-  Lemma fmap_stateT_id {S} : ∀ A, fmap_stateT (S:=S) (id (A:=A)) = id.
-  Proof.
-    unfold fmap_stateT. intros. ext. ext. autorewrite with soundness.
-    rewrite <- bind_id_right. f_equal; ext. destruct x1.
-    reflexivity.
-  Qed.
-
-  Lemma fmap_stateT_compose {S} : ∀ {A B C : Type} (f : A → B) (g : B → C),
-  fmap_stateT (S:=S) (f ∘ g) = fmap_stateT f ∘ fmap_stateT g.
-  Proof.
-    intros. unfold fmap_stateT. unfold compose.
-    ext. ext. autorewrite with soundness. f_equal; ext.
-    destruct x1. autorewrite with soundness. reflexivity.
-  Qed.
-  Arguments fmap_stateT_compose [S A B C] f g.
-
-  Global Instance functor_stateT S : Functor (StateT S M) :=
-  {
-    fmap := @fmap_stateT S;
-    fmap_id := @fmap_stateT_id S;
-    fmap_compose := @fmap_stateT_compose S;
-  }. 
-End Functor_StateT.
-Hint Unfold fmap_stateT : soundness.
-
-Section Applicative_StateT.
-  Context {M} `{M_monad : Monad M}.
-  Context {S : Type}.
-
-  Definition pure_stateT {A} (x : A) : StateT S M A :=
-    fun s => pure (x, s).
-  Arguments pure_stateT [A] x.
-
-  Definition app_stateT {A B}
-    (sf : StateT S M (A -> B)) (sa : StateT S M A) : StateT S M B :=
-    fun st : S =>
-    bindM (sf st) (fun '(f, stf) =>
-      bindM (sa stf) (fun '(a, sta) =>
-        pure (f a, sta))).
-  Arguments app_stateT [A B] sf sa.
-  Hint Unfold pure_stateT app_stateT : soundness.
-
-  Lemma app_stateT_id : ∀ (A : Type) (x : StateT S M A), 
-    app_stateT (pure_stateT (id (A:=A))) x = x.
-  Proof.
-    intros. unfold app_stateT, pure_stateT.
-    ext. autorewrite with soundness. rewrite <- bind_id_right.
-    f_equal. ext. destruct x1. reflexivity.
-  Qed.
-  Arguments app_stateT_id [A] x.
-
-  Lemma app_stateT_homomorphism : ∀ (A B : Type) (f : A → B) (x : A),
-  app_stateT (pure_stateT f) (pure_stateT x) = pure_stateT (f x).
-  Proof.
-    intros. unfold app_stateT, pure_stateT. ext. autorewrite with soundness.
-    reflexivity.
-  Qed.
-  Arguments app_stateT_homomorphism [A B] f x.
-
-  Lemma app_stateT_interchange : ∀ (A B : Type) 
-    (u : StateT S M (A → B)) (y : A),
-  app_stateT u (pure_stateT y) = app_stateT (pure_stateT (λ f : A → B, f y)) u.
-  Proof.
-    intros. autounfold with soundness. ext. autorewrite with soundness.
-    f_equal; ext. destruct x0. autorewrite with soundness. reflexivity.
-  Qed.
-  Arguments app_stateT_interchange [A B] u y.
-
-  Lemma app_stateT_compose : ∀ (A B C : Type) (u : StateT S M (B → C)) 
-    (v : StateT S M (A → B)) (w : StateT S M A),
-  app_stateT u (app_stateT v w) =
-  app_stateT (app_stateT (app_stateT (pure_stateT compose) u) v) w.
-  Proof.
-    intros. autounfold with soundness. ext. autorewrite with soundness.
-    f_equal; ext. destruct x0. autorewrite with soundness.
-    f_equal; ext. destruct x0. autorewrite with soundness.
-    f_equal; ext. destruct x0. autorewrite with soundness. unfold compose.
-    reflexivity.
-  Qed.
-  Arguments app_stateT_compose [A B C] u v w.
-
-  Lemma app_stateT_fmap : ∀ (A B : Type) (f : A → B) (x : StateT S M A),
-    fmap f x = app_stateT (pure_stateT f) x.
-  Proof.
-    simple_solve.
-  Qed.
-
-  Lemma pure_stateT_inj : ∀ (A : Type) (x y : A),
-    pure_stateT x = pure_stateT y → x = y.
-  Proof. 
-    intros A x y Hfun_eq. unfold pure_stateT in Hfun_eq.
-    eapply equal_f in Hfun_eq. apply pure_inj in Hfun_eq.
-    inversion Hfun_eq. reflexivity.
-  Admitted.
-
-  Global Instance applicative_stateT : Applicative (StateT S M) :=
-  {
-    pure := pure_stateT;
-    pure_inj := pure_stateT_inj;
-    app := app_stateT;
-    app_id := app_stateT_id;
-    app_homomorphism := app_stateT_homomorphism;
-    app_interchange := app_stateT_interchange;
-    app_compose := app_stateT_compose;
-    app_fmap := app_stateT_fmap;
-  }. 
-End Applicative_StateT.
-Hint Unfold pure_stateT app_stateT : soundness.
-
 Section Monad_StateT.
   Context {M} `{M_monad : Monad M}.
   Context {S : Type}.
+
+  Definition return_stateT {A} (a : A) :=
+    λ st : S, returnM (a, st).
+  Hint Unfold return_stateT : soundness.
+
+  Lemma return_stateT_inj : ∀ A (x y : A),
+    return_stateT x = return_stateT y → x = y.
+  Proof.
+    intros A x y Heq. unfold return_stateT in Heq.
+  Admitted.
 
   Definition bind_stateT {A B} (MA : StateT S M A) 
     (f : A -> StateT S M B) : StateT S M B :=
@@ -1183,7 +382,7 @@ Section Monad_StateT.
   Hint Unfold bind_stateT : soundness.
 
   Lemma bind_stateT_id_left : ∀ (A B : Type) (f : A → StateT S M B) (a : A), 
-    bind_stateT (pure_stateT a) f = f a.
+    bind_stateT (return_stateT a) f = f a.
   Proof.
     autounfold with soundness. intros. ext. 
     rewrite bind_id_left. reflexivity.
@@ -1191,7 +390,7 @@ Section Monad_StateT.
   Arguments bind_stateT_id_left [A B] f a.
 
   Lemma bind_stateT_id_right : ∀ (A : Type) (MA : StateT S M A), 
-    bind_stateT MA pure_stateT = MA.
+    bind_stateT MA return_stateT = MA.
   Proof.
     intros. autounfold with soundness. ext.
     rewrite <- bind_id_right. f_equal. ext. destruct x0.
@@ -1210,46 +409,12 @@ Section Monad_StateT.
   Qed.
   Arguments bind_stateT_assoc [A B C] MA f g.
   
-  Lemma bind_stateT_app : ∀ (A B : Type) (mf : StateT S M (A → B)) 
-    (ma : StateT S M A), 
-    app_stateT mf ma =
-  bind_stateT mf (λ f : A → B,  bind_stateT ma (λ a : A, (f ∘ pure_stateT) a)).
-  Proof.
-    autounfold with soundness. intros.
-    ext. f_equal.
-  Qed.
-  Arguments bind_stateT_app [A B] mf ma.
-
-  Lemma bind_stateT_fmap :  ∀ (A B C : Type) (f : A → B) (x : StateT S M A) 
-    (g : B → StateT S M C),
-    bind_stateT (fmap_stateT f x) g = bind_stateT x (f ∘ g).
-  Proof.
-    autounfold with soundness. intros. ext. autorewrite with soundness.
-    f_equal; ext. destruct x1. autorewrite with soundness.
-    reflexivity.
-  Qed.
-  Arguments bind_stateT_fmap [A B C] f x g.
-
-  Lemma bind_stateT_pass : ∀ (A B : Type) (ma : StateT S M A) 
-    (mb : StateT S M B),
-  ma >> mb = bind_stateT ma (λ _ : A, mb).
-  Proof.
-    intros. simpl. autounfold with soundness. 
-    ext. autorewrite with soundness. f_equal.
-    ext. destruct x0. autorewrite with soundness. rewrite <- bind_id_right.
-    f_equal. ext. destruct x0. unfold const. reflexivity.
-  Qed.
-  Arguments bind_stateT_pass [A B] ma mb.
-
   Global Instance monad_stateT : Monad (StateT S M) :=
   {
-    bindM := bind_stateT;
+    returnM_inj := return_stateT_inj;
     bind_id_left := bind_stateT_id_left;
     bind_id_right := bind_stateT_id_right;
     bind_assoc := bind_stateT_assoc;
-    bind_app := bind_stateT_app;
-    bind_fmap := bind_stateT_fmap;
-    bind_pass := bind_stateT_pass;
   }. 
 End Monad_StateT.
 Hint Unfold bind_stateT : soundness.
@@ -1259,12 +424,12 @@ Section MonadT_StateT.
   Context {S : Type}.
 
   Definition lift_stateT {A} (MA : M A) : StateT S M A :=
-    fun st => bindM MA (fun a => pure (a, st)).
+    fun st => bindM MA (fun a => returnM (a, st)).
   Arguments lift_stateT [A] MA.
   Hint Unfold lift_stateT : soundness.
   
   Lemma lift_stateT_pure : ∀ (A : Type) (x : A), 
-    lift_stateT (pure x) = pure_stateT x.
+    lift_stateT (returnM x) = return_stateT x.
   Proof.
     intros. autounfold with soundness. ext.
     autorewrite with soundness. reflexivity.
@@ -1283,7 +448,7 @@ Section MonadT_StateT.
   Global Instance monadT_stateT : MonadT (StateT S) :=
   {
     liftT := lift_stateT;
-    lift_pure := lift_stateT_pure;
+    lift_return := lift_stateT_pure;
     lift_bind := lift_stateT_bind;
   }. 
 End MonadT_StateT.
