Classes/Monad.v
@@ -6,31 +6,23 @@ Implicit Type M : Type → Type.
 Implicit Type T : (Type → Type) → Type → Type.
 Implicit Type A B C D : Type.
 
-Class Monad M `{M_applicative : Applicative M}: Type :=
+Class Monad M : Type :=
 {
+  returnM : ∀ {A}, A → M A;
+  returnM_inj : ∀ {A} (x y : A), returnM x = returnM y → x = y;
   bindM : ∀ {A B}, M A  → (A → M B) → M B;
   bind_id_left : ∀ {A B} (f : A → M B) (a : A), 
-    bindM (pure a) f = f a;
+    bindM (returnM a) f = f a;
   bind_id_right : ∀ {A} (MA : M A),
-    bindM MA pure = MA;
+    bindM MA returnM = MA;
   bind_assoc : ∀ {A B C} (MA : M A) (f : A → M B) (g : B → M C),
     bindM (bindM MA f) g = bindM MA (λ a, bindM (f a) g);
-  bind_app : ∀ {A B} (mf : M (A → B)) (ma : M A),
-    mf <*> ma = bindM mf (λ f, bindM ma (λ a, (f ∘ pure) a));
-  bind_fmap : ∀ {A B C} (f : A → B) (x : M A) (g : B → M C),
-    bindM (f <$> x) g = bindM x (f ∘ g);
-  bind_pass : ∀ {A B} (ma : M A) (mb : M B), ma >> mb = bindM ma (λ _, mb);
 }.
 Arguments bindM : simpl never.
+Arguments returnM: simpl never.
 Hint Unfold bindM : soundness.
 
-Hint Rewrite @bind_id_left @bind_id_right @bind_assoc @bind_app : soundness.
-
-Definition skip {M} `{M_monad : Monad M} := pure tt.
-
-Definition composeM {M : Type → Type} `{M_monad : Monad M}
-  {A B C} (f : A → M B) (g : B → M C) (x : A) : M C :=
-  bindM (f x) g.
+Hint Rewrite @bind_id_left @bind_id_right @bind_assoc : soundness.
 
 Ltac solve_monad := repeat (simplify; simple_solve;
   match goal with
@@ -40,84 +32,10 @@ Ltac solve_monad := repeat (simplify; simple_solve;
   end).
 
 Notation "x >>= y" := (bindM x y) (at level 40, left associativity).
-Notation "x >=> y" := (composeM x y) (at level 40, left associativity).
-
-Section laws_and_methods.
-  Context {M} `{M_monad : Monad M}.
-
-  Definition join {A} (x : M (M A)) : M A := bindM x id.
-
-  Lemma join_fmap {A : Type} (x : M(M(M(A)))) : 
-    join (join <$> x) = join (join x).
-  Proof.
-    unfold join. rewrite bind_fmap. rewrite bind_assoc.
-    f_equal.
-  Qed.
-
-  Lemma join_return {A} (x : M A) : 
-    join (fmap pure x) = join (pure x).
-  Proof.
-    unfold join. rewrite bind_id_left. 
-    rewrite id_refl. unfold id. rewrite bind_fmap.
-    unfold compose. apply bind_id_right. 
-  Qed.
- 
-  Lemma fmap_bind : ∀ {A B C} (x : M A) (f : A → M B) (g : B → C),
-    fmap g (bindM x f) = bindM x (λ a, fmap g (f a)).
-  Proof. 
-    intros. rewrite app_fmap. rewrite bind_app. rewrite bind_id_left.
-    rewrite bind_assoc. f_equal. ext. rewrite app_fmap.
-    rewrite bind_app. rewrite bind_id_left. f_equal.
-  Qed.
-
-  Lemma fmap_bind_pure : ∀ {A B} (f : A → B) (x : M A),
-    fmap f x = bindM x (λ a, (f ∘ pure) a).
-  Proof.
-    intros. rewrite <- bind_fmap. rewrite bind_id_right. reflexivity.
-  Qed.
-
-  Lemma composeM_assoc : ∀ {A B C D} 
-    (f : A → M B) (g : B → M C) (h : C → M D),
-    f >=> (g >=> h) = (f >=> g) >=> h.
-  Proof.
-    intros. unfold composeM. ext. rewrite bind_assoc. f_equal.
-  Qed.
-
-  Lemma composeM_pure_left : ∀ {A B} (f : A → M B),
-    pure >=> f = f.
-  Proof.
-    intros. unfold composeM. ext. rewrite bind_id_left. reflexivity.
-  Qed.
-
-  Lemma composeM_pure_right : ∀ {A B} (f : A → M B),
-    f >=> pure = f.
-  Proof.
-    intros. unfold composeM. ext. rewrite bind_id_right. reflexivity.
-  Qed.
-
-  Lemma composeM_comp : ∀ {A B C} (f : A → B) (g : B → M C),
-    (f ∘ pure) >=> g = f ∘ g.
-  Proof.
-    intros. unfold composeM, compose. ext.
-    rewrite bind_id_left. reflexivity.
-  Qed.
-
-  Lemma composeM_fmap : ∀ {A B C} (f : A → M B) (g : B → C),
-    f >=> (g ∘ pure) = f ∘ fmap g.
-  Proof.
-    intros. unfold composeM. ext. rewrite <- bind_fmap. rewrite bind_id_right.
-    reflexivity. 
-  Qed.
-
-End laws_and_methods.
-Hint Rewrite @bind_fmap @fmap_bind @fmap_bind_pure : soundness.
-Hint Rewrite <- @bind_pass : soundness.
-
-Notation "x >>= y" := (bindM x y) (at level 40, left associativity).
-Notation "x >=> y" := (composeM x y) (at level 40, left associativity).
 Notation "x '<-' y ; z" := (bindM y (λ x, z))
   (at level 20, y at level 100, z at level 200, only parsing).
-
+Notation "x ;; z" := (bindM x (λ _, z))
+    (at level 100, z at level 200, only parsing, right associativity).
 
 Section MonadTransformer.
   Context {M} `{M_monad : Monad M}.
@@ -125,10 +43,10 @@ Section MonadTransformer.
   Class MonadT T `{TM_monad : Monad (T M)} : Type :=
   {
     liftT : ∀ {A}, M A → T M A;
-    lift_pure : ∀  {A} (x : A), liftT (pure x) = pure x;
+    lift_return : ∀  {A} (x : A), liftT (returnM x) = returnM x;
     lift_bind : ∀ {A B} (x : M A) (f : A → M B),
       liftT (x >>= f) = liftT x >>= (f ∘ liftT);
   }.
 End MonadTransformer.
 Hint Unfold liftT : soundness.
-Hint Rewrite @lift_pure @lift_bind : soundness.
+Hint Rewrite @lift_return @lift_bind : soundness.
