Classes/Monad/MonadExcept.v
@@ -1,5 +1,4 @@
 Require Export Base.
-Require Import Classes.Applicative.
 Require Import Classes.Monad.
 Require Import Classes.Monad.MonadFail.
 
@@ -12,9 +11,8 @@ Class MonadExcept M `{M_fail : MonadFail M} A := {
   catch_right : ∀ (x : M A), catch x fail = x;
   catch_assoc : ∀ (x y z: M A),
     catch x (catch y z) = catch (catch x y) z;
-  catch_pure : ∀ (x : M A) (a : A),
-    catch (pure a) x = pure a;
+  catch_return : ∀ (x : M A) (a : A),
+    catch (returnM a) x = returnM a;
 }.
 Arguments catch : simpl never.
-
-Hint Rewrite @catch_left @catch_right @catch_pure : soundness.
+Hint Rewrite @catch_left @catch_right @catch_return : soundness.
