Classes/SoundMonad.v
@@ -1,8 +1,6 @@
 Require Export Base.
 Require Import Classes.PreorderedSet.
 Require Import Classes.Galois.
-Require Import Classes.Functor.
-Require Import Classes.Applicative.
 Require Import Classes.Monad.
 Require Import Classes.Monad.MonadFail.
 Require Import Instances.Galois.
@@ -14,15 +12,11 @@ Section sound_monad.
 
   Class SoundMonad : Type :=
   {
-    fmap_sound : ∀ (A A' B B' : Type) `{Galois A A', Galois B B'},
-      gamma (fmap (M:=M') (A:=A') (B:=B')) (fmap (M:=M) (A:=A) (B:=B));
-    pure_sound : ∀ (A A' : Type) `{Galois A A'},
-      gamma (pure (M:=M') (A:=A')) (pure (M:=M) (A:=A));
-    app_sound : ∀ (A A' B B' : Type) `{Galois A A', Galois B B'},
-      gamma (app (M:=M') (A:=A') (B:=B')) (app (M:=M) (A:=A) (B:=B));
+    return_sound : ∀ (A A' : Type) `{Galois A A'},
+      gamma (returnM (M:=M') (A:=A')) (returnM (M:=M) (A:=A));
     bind_sound : ∀ (A A' B B' : Type) `{Galois A A', Galois B B'},
       gamma (bindM (M:=M') (A:=A') (B:=B')) (bindM (M:=M) (A:=A) (B:=B));
     gamma_fail : ∀ (A A' : Type) `{Galois A A'} (m : M A), gamma fail m;
   }.
 End sound_monad.
-Hint Resolve fmap_sound pure_sound app_sound bind_sound gamma_fail : soundness.
+Hint Resolve return_sound bind_sound gamma_fail : soundness.
