Instances/IsBool/Boolean.v
@@ -4,27 +4,26 @@ Require Import Classes.Monad.MonadFail.
 Require Import Language.Statements.
 Require Import Types.Stores.
 Require Import Instances.Monad.
-Require Import Classes.Applicative.
 
 Generalizable Variable M.
 
 Definition ensure_bool `{M_monad : MonadFail M} (v : cvalue) : M bool :=
   match v with
-  | VBool b => pure b
+  | VBool b => returnM b
   | _ => fail
   end.
 
 Definition build_boolean `{M_monad : Monad M} (b : bool) : M cvalue :=
-  pure (VBool b).
+  returnM (VBool b).
 
 Definition extract_boolean `{M_monad : Monad M} (b : bool) : M bool :=
-  pure b.
+  returnM b.
 
 Definition andbM `{M_monad : Monad M} (b c : bool) : M bool := 
-  pure (andb b c).
+  returnM (andb b c).
 
 Definition negbM `{M_monad : Monad M} (b : bool) : M bool := 
-  pure (negb b).
+  returnM (negb b).
 
 Definition eval_if {A} `{M_monad : Monad M} (b : bool) (st1 st2 : M A) : M A :=
   if b then st1 else st2.
