Instances/IsNat/Interval.v
@@ -11,28 +11,28 @@ Implicit Type M : Type → Type.
 Generalizable Variable M.
 
 Definition extract_interval `{M_monad : Monad M} (n : nat) : M interval := 
-  pure (n, n).
+  returnM (n, n).
 
 Definition ensure_interval `{M_fail : MonadFail M} (v : avalue) : M interval :=
   match v with
-  | VInterval i => pure i
+  | VInterval i => returnM i
   | _ => fail
   end.
 
 Definition iplusM `{M_monad : Monad M} (i j : interval) : M interval := 
-  pure (iplus i j).
+  returnM (iplus i j).
 
 Definition imultM `{M_monad : Monad M} (i j : interval) : M interval :=
-  pure (imult i j).
+  returnM (imult i j).
 
 Definition ieqM `{M_monad : Monad M} (i j : interval) : M abstr_bool :=
-  pure (ieqb i j).
+  returnM (ieqb i j).
 
 Definition ileM `{M_monad : Monad M} (i j : interval) : M abstr_bool := 
-  pure (ileqb i j).
+  returnM (ileqb i j).
 
 Definition build_interval `{M_monad : Monad M} (i : interval) : M avalue :=
-  pure (VInterval i).  
+  returnM (VInterval i).  
 
 Global Instance isnat_interval `{M_fail : MonadFail M} :
   IsNat M avalue abstr_bool interval :=
