Instances/Store.v
@@ -5,21 +5,19 @@ Require Import Classes.Store.
 Require Import Types.Stores.
 Require Import Instances.Monad.
 Require Import Classes.Monad.
-Require Import Classes.Applicative.
-Require Import Classes.Functor.
 
 Section store_stateT_concrete. 
   Context (M : Type -> Type) `{M_monad : Monad M}.
 
-  Definition stateT_get (S : Type) := fun s : S => pure (s, s).
+  Definition stateT_get (S : Type) := fun s : S => returnM (s, s).
 
-  Definition stateT_put (S : Type) := fun s : S => fun _ : S => pure (tt, s).
+  Definition stateT_put (S : Type) := fun s : S => fun _ : S => returnM (tt, s).
 
   Definition retrieve_concrete (x : string) : StateT store M cvalue :=
-    fun s : store => pure(s x, s).
+    fun s : store => returnM (s x, s).
 
   Definition update_concrete (x : string) (v : cvalue) : StateT store M store :=
-    fun s : store => let s' := t_update s x v in pure(s', s').
+    fun s : store => let s' := t_update s x v in returnM (s', s').
 
   Global Instance store_stateT (S : Type) : 
   Store store (StateT store M) cvalue :=
@@ -34,13 +32,13 @@ End store_stateT_concrete.
 Section store_stateT_abstract.
   Context (M : Type -> Type) `{M_monad : Monad M}.
 
-  Definition get_abstract (S : Type) := fun s : S => pure (s, s).
-  Definition put_abstract (S : Type) := fun s : S => fun _ : S => pure (tt, s).
+  Definition get_abstract (S : Type) := fun s : S => returnM (s, s).
+  Definition put_abstract (S : Type) := fun s : S => fun _ : S => returnM (tt, s).
   Definition retrieve_abstract (x : string) : StateT abstract_store M avalue :=
-    fun s : abstract_store => pure (s x, s).
+    fun s : abstract_store => returnM (s x, s).
   Definition update_abstract (x : string) (v : avalue) : 
     StateT abstract_store M abstract_store :=
-    fun s : abstract_store => let s' := t_update s x v in pure(s', s').
+    fun s : abstract_store => let s' := t_update s x v in returnM (s', s').
 
   Global Instance store_stateT_abstract (S : Type) : 
     Store abstract_store (StateT abstract_store M) avalue :=
@@ -60,7 +58,7 @@ Section store_maybeT.
   Store S (MaybeT M) V :=
   {
     get := liftT get;
-    put := fun s => put s ;; pure (Just tt);
+    put := fun s => put s ;; returnM (Just tt);
     retrieve := fun x : string => liftT (retrieve x);
     update := fun x v => liftT (update x v);
   }.
@@ -72,8 +70,8 @@ Section store_maybeAT.
   Global Instance store_maybeAT (S : Type) `{Store S M V} :
   Store S (MaybeAT M) V :=
   {
-    get := fmap JustA get;
-    put := fun s => put s ;; pure (JustA tt);
+    get := liftT get;
+    put := fun s => put s ;; returnM (JustA tt);
     retrieve := fun x => liftT (retrieve x);
     update := fun x v => liftT (update x v);
   }.
